@prefix owl: <http://www.w3.org/2002/07/owl#> .
@prefix rdf: <http://www.w3.org/1999/02/22-rdf-syntax-ns#> .
@prefix xml: <http://www.w3.org/XML/1998/namespace> .
@prefix xsd: <http://www.w3.org/2001/XMLSchema#> .
@prefix rdfs: <http://www.w3.org/2000/01/rdf-schema#> .
@base <http://www.w3.org/2002/07/owl#> .

[ rdf:type owl:Ontology ;
   <http://purl.org/dc/elements/1.1/contributor> "Jay Jay Billings" ;
   <http://purl.org/dc/elements/1.1/creator> <https://www.eclipse.org/ice> ;
   <http://purl.org/dc/elements/1.1/format> "application/rdf+xml" ;
   <http://purl.org/dc/elements/1.1/language> "en" ;
   <http://purl.org/dc/elements/1.1/title> """The Eclipse Integrated Environment Workflow
			Ontology"""@en ;
   owl:versionInfo "1.0"
 ] .

#################################################################
#    Annotation properties
#################################################################

###  http://purl.org/dc/elements/1.1/contributor
<http://purl.org/dc/elements/1.1/contributor> rdf:type owl:AnnotationProperty .


###  http://purl.org/dc/elements/1.1/creator
<http://purl.org/dc/elements/1.1/creator> rdf:type owl:AnnotationProperty .


###  http://purl.org/dc/elements/1.1/format
<http://purl.org/dc/elements/1.1/format> rdf:type owl:AnnotationProperty .


###  http://purl.org/dc/elements/1.1/language
<http://purl.org/dc/elements/1.1/language> rdf:type owl:AnnotationProperty .


###  http://purl.org/dc/elements/1.1/title
<http://purl.org/dc/elements/1.1/title> rdf:type owl:AnnotationProperty .


#################################################################
#    Object Properties
#################################################################

###  https://www.eclipse.org/ice/workflows#dependsOn
<https://www.eclipse.org/ice/workflows#dependsOn> rdf:type owl:ObjectProperty ;
                                                  rdfs:subPropertyOf owl:topObjectProperty ;
                                                  rdfs:domain <https://www.eclipse.org/ice/workflows#Task> ,
                                                              <https://www.eclipse.org/ice/workflows#WorkflowDescription> ;
                                                  rdfs:range <https://www.eclipse.org/ice/workflows#Task> ,
                                                             <https://www.eclipse.org/ice/workflows#WorkflowDescription> ;
                                                  rdfs:comment """This property indicates that the task (domain) depends on the successful execution of the range, which is another task or set of tasks.

It is possible to declare multiple instances of this object property such that one task will depend on the successful execution of multiple tasks.""" ;
                                                  rdfs:label "depends On" .


###  https://www.eclipse.org/ice/workflows#executes
<https://www.eclipse.org/ice/workflows#executes> rdf:type owl:ObjectProperty ;
                                                 rdfs:domain <https://www.eclipse.org/ice/workflows#WorkflowDescription> ;
                                                 rdfs:range <https://www.eclipse.org/ice/workflows#Task> ;
                                                 rdfs:comment "This property links a workflow description to a task that it should execute." ;
                                                 rdfs:label "executes" .


###  https://www.eclipse.org/ice/workflows#hasAction
<https://www.eclipse.org/ice/workflows#hasAction> rdf:type owl:ObjectProperty ;
                                                  rdfs:subPropertyOf owl:topObjectProperty ;
                                                  rdfs:domain <https://www.eclipse.org/ice/workflows#ConditionalAction> ,
                                                              <https://www.eclipse.org/ice/workflows#Task> ;
                                                  rdfs:range <https://www.eclipse.org/ice/workflows#Action> ;
                                                  rdfs:comment "This object property denotes that the task (domain) uses the action (range) to which it points." ;
                                                  rdfs:label "has Action" .


###  https://www.eclipse.org/ice/workflows#hasActionTarget
<https://www.eclipse.org/ice/workflows#hasActionTarget> rdf:type owl:ObjectProperty ;
                                                        rdfs:domain <https://www.eclipse.org/ice/workflows#Action> ;
                                                        rdfs:comment "This tag describes the target (program, function, web service, etc.) that the action should execute. Its domain is tied to Action, but its range is open to accommodate what ever the type of the target is."@en ;
                                                        rdfs:label "has Action Target"@en .


###  https://www.eclipse.org/ice/workflows#hasActionType
<https://www.eclipse.org/ice/workflows#hasActionType> rdf:type owl:ObjectProperty ;
                                                      rdfs:domain <https://www.eclipse.org/ice/workflows#Action> ;
                                                      rdfs:range <https://www.eclipse.org/ice/workflows#ActionType> ;
                                                      rdfs:comment "This property links a concrete action type to the subject, which must be an action instance." ;
                                                      rdfs:label "has Action Type" .


###  https://www.eclipse.org/ice/workflows#hasCondition
<https://www.eclipse.org/ice/workflows#hasCondition> rdf:type owl:ObjectProperty ;
                                                     rdfs:domain <https://www.eclipse.org/ice/workflows#Task> ;
                                                     rdfs:range <https://www.eclipse.org/ice/workflows#ConditionalAction> ;
                                                     rdfs:comment "This property indicates that the conditional task (domain) is subject to the completion only if the conditional action (range) executes successfully." ;
                                                     rdfs:label "has Condition" .


###  https://www.eclipse.org/ice/workflows#hasProperties
<https://www.eclipse.org/ice/workflows#hasProperties> rdf:type owl:ObjectProperty ;
                                                      rdfs:subPropertyOf owl:topObjectProperty ;
                                                      rdfs:domain <https://www.eclipse.org/ice/workflows#Task> ;
                                                      rdfs:comment "This property indicates that the task (domain) has the properties described by the range. The range is open because the type of the properties may be undefined." ;
                                                      rdfs:label "has Properties" .


###  https://www.eclipse.org/ice/workflows#onStateChange
<https://www.eclipse.org/ice/workflows#onStateChange> rdf:type owl:ObjectProperty ;
                                                      rdfs:domain <https://www.eclipse.org/ice/workflows#Task> ;
                                                      rdfs:range <https://www.eclipse.org/ice/workflows#StateChangeAction> ;
                                                      rdfs:comment "This property links a task (domain) to a state change action (range) that it should execute when its state changes." ;
                                                      rdfs:label "on State Change" .


###  https://www.eclipse.org/ice/workflows#targetMethod
<https://www.eclipse.org/ice/workflows#targetMethod> rdf:type owl:ObjectProperty ;
                                                     rdfs:subPropertyOf owl:topObjectProperty ;
                                                     rdfs:domain <https://www.eclipse.org/ice/workflows#JavaClass> ;
                                                     rdfs:comment "This property identifies the target method that should be used to launch the action." ;
                                                     rdfs:label "target method" .


#################################################################
#    Data properties
#################################################################

###  https://www.eclipse.org/ice/workflows#hasHost
<https://www.eclipse.org/ice/workflows#hasHost> rdf:type owl:DatatypeProperty ;
                                                rdfs:subPropertyOf owl:topDataProperty ;
                                                rdfs:domain <https://www.eclipse.org/ice/workflows#Task> ,
                                                            <https://www.eclipse.org/ice/workflows#WorkflowDescription> ;
                                                rdfs:range xsd:anyURI ;
                                                rdfs:comment "This property describes the host on which a task or workflow should be executed." ;
                                                rdfs:label "has Host" .


###  https://www.eclipse.org/ice/workflows#hasState
<https://www.eclipse.org/ice/workflows#hasState> rdf:type owl:DatatypeProperty ;
                                                 rdfs:domain <https://www.eclipse.org/ice/workflows#Task> ,
                                                             <https://www.eclipse.org/ice/workflows#WorkflowDescription> ;
                                                 rdfs:range [ rdf:type rdfs:Datatype ;
                                                              owl:oneOf [ rdf:type rdf:List ;
                                                                          rdf:first "Executing" ;
                                                                          rdf:rest [ rdf:type rdf:List ;
                                                                                     rdf:first "Failed" ;
                                                                                     rdf:rest [ rdf:type rdf:List ;
                                                                                                rdf:first "Finished" ;
                                                                                                rdf:rest [ rdf:type rdf:List ;
                                                                                                           rdf:first "Initialized" ;
                                                                                                           rdf:rest [ rdf:type rdf:List ;
                                                                                                                      rdf:first "Ready" ;
                                                                                                                      rdf:rest [ rdf:type rdf:List ;
                                                                                                                                 rdf:first "Reviewing" ;
                                                                                                                                 rdf:rest [ rdf:type rdf:List ;
                                                                                                                                            rdf:first "Waiting" ;
                                                                                                                                            rdf:rest [ rdf:type rdf:List ;
                                                                                                                                                       rdf:first "WaitingForInfo" ;
                                                                                                                                                       rdf:rest rdf:nil
                                                                                                                                                     ]
                                                                                                                                          ]
                                                                                                                               ]
                                                                                                                    ]
                                                                                                         ]
                                                                                              ]
                                                                                   ]
                                                                        ]
                                                            ] ;
                                                 rdfs:comment """This data property describes the present state of the task or workflow.

Initialized

This pseudostate indicates that the state machine has fully initialized. In practice, full and successful initialization results in an immediate local transition to Ready.

Failed

This state indicates that an unexpected failure happened while executing the task.

Reviewing

The Reviewing state is entered when a task needs to spend a large amount of time to review information received for pre-, post-, or in-situ processing that is required to execute the task. Once the review is complete, the task will transition into the Executing state in the ideal primary flow.

Waiting

Tasks in the waiting state are waiting on resources to be properly allocated, including either compute or data resources.

WaitingForInfo

Tasks in the WaitingForInfo state are waiting on information from an external agent.

Finished

This is the terminal state for the task and indicates that it has been completely executed.

Executing

This state indicates that the task is presently executing the work assigned to it.

Ready

The ready state indicates that the task can be executed and that all initialization has completed, or that execution has finished and the task is ready to be executed again.""" ;
                                                 rdfs:label "has State" .


###  https://www.eclipse.org/ice/workflows#lowerBound
<https://www.eclipse.org/ice/workflows#lowerBound> rdf:type owl:DatatypeProperty ;
                                                   rdfs:range xsd:integer ;
                                                   rdfs:comment "An upper bound on a range between this bound and a minimum, lower bound, with a set of discrete steps of finite size between the two bounds." ;
                                                   rdfs:label "Lower Bound" .


###  https://www.eclipse.org/ice/workflows#stepSize
<https://www.eclipse.org/ice/workflows#stepSize> rdf:type owl:DatatypeProperty ;
                                                 rdfs:subPropertyOf owl:topDataProperty ;
                                                 rdfs:range xsd:integer ;
                                                 rdfs:comment "The step size between upper and lower bounds for any such configuration." ;
                                                 rdfs:label "Step Size" .


###  https://www.eclipse.org/ice/workflows#upperBound
<https://www.eclipse.org/ice/workflows#upperBound> rdf:type owl:DatatypeProperty ;
                                                   rdfs:range xsd:integer ;
                                                   rdfs:comment "A lower bound on a range between this bound and a maximum, upper bound, with a set of discrete steps of finite size between the two bounds." ;
                                                   rdfs:label "Upper bound" .


#################################################################
#    Classes
#################################################################

###  https://www.eclipse.org/ice/data#Identifiable
<https://www.eclipse.org/ice/data#Identifiable> rdf:type owl:Class .


###  https://www.eclipse.org/ice/workflows#Action
<https://www.eclipse.org/ice/workflows#Action> rdf:type owl:Class ;
                                               rdfs:comment "This is an action that can be executed in a task of the workflow."@en ;
                                               rdfs:label "Action"@en .


###  https://www.eclipse.org/ice/workflows#ActionType
<https://www.eclipse.org/ice/workflows#ActionType> rdf:type owl:Class ;
                                                   rdfs:comment "This resource defines the type of the action that will be executed. It distinguishes between types of actions such as shell functions, user input, waiting, etc." ;
                                                   rdfs:label "Action Type" .


###  https://www.eclipse.org/ice/workflows#BasicActionType
<https://www.eclipse.org/ice/workflows#BasicActionType> rdf:type owl:Class ;
                                                        rdfs:subClassOf <https://www.eclipse.org/ice/workflows#ActionType> ;
                                                        rdfs:comment "The Basic Action Type is the base class for basic actions that are typically considered native actions of workflow engines that execute workflows. This includes actions such as moving files or doing simple reductions." ;
                                                        rdfs:label "Basic Action Type" .


###  https://www.eclipse.org/ice/workflows#BooleanCondition
<https://www.eclipse.org/ice/workflows#BooleanCondition> rdf:type owl:Class ;
                                                         rdfs:subClassOf <https://www.eclipse.org/ice/workflows#Condition> ;
                                                         rdfs:comment "Boolean Conditions evaluate boolean statements, such as \"if\" statements." ;
                                                         rdfs:label "Boolean Condition" .


###  https://www.eclipse.org/ice/workflows#CWLTool
<https://www.eclipse.org/ice/workflows#CWLTool> rdf:type owl:Class ;
                                                rdfs:subClassOf <https://www.eclipse.org/ice/workflows#ShellScript> ;
                                                rdfs:comment "This node represents a Common Workflow Language (CWL) Tool, which is a description of a command line tool used in CWL workflows." ;
                                                rdfs:label "Common Workflow Language Tool" .


###  https://www.eclipse.org/ice/workflows#Condition
<https://www.eclipse.org/ice/workflows#Condition> rdf:type owl:Class ;
                                                  rdfs:subClassOf <https://www.eclipse.org/ice/workflows#ActionType> ;
                                                  rdfs:comment """Conditional Actions Types indicate that the action described by this type executes for the purpose of evaluating some logical condition, such as a boolean statement, a loop, a cycle, or waiting (polling, checking) for feedback from an external agent.

The targetMethod object property of a Condition must always point to one of the functional (i.e. - non-conditional) action types.""" ;
                                                  rdfs:label "Condition" .


###  https://www.eclipse.org/ice/workflows#ConditionalAction
<https://www.eclipse.org/ice/workflows#ConditionalAction> rdf:type owl:Class ;
                                                          rdfs:subClassOf <https://www.eclipse.org/ice/workflows#Action> ;
                                                          rdfs:comment """Conditional Actions are actions that execute conditionally for either conditional tasks (i.e. - as part of the workflow) or as alternative execution flows when the task enters a different state.

Conditional actions assigned to tasks indicate that the primary action of the task should be executed according to the conditional action type until the condition action evaluates to true.""" ;
                                                          rdfs:label "Conditional Action" .


###  https://www.eclipse.org/ice/workflows#Cycle
<https://www.eclipse.org/ice/workflows#Cycle> rdf:type owl:Class ;
                                              rdfs:subClassOf <https://www.eclipse.org/ice/workflows#Condition> ;
                                              rdfs:comment "A Cycle describes an action that exits when a condition describing the end of a cycle has been met. Where a loop action type describes execution over a range, a cyclic action type checks for the completion of a task cycle." ;
                                              rdfs:label "Cycle" .


###  https://www.eclipse.org/ice/workflows#Executable
<https://www.eclipse.org/ice/workflows#Executable> rdf:type owl:Class ;
                                                   rdfs:subClassOf <https://www.eclipse.org/ice/workflows#ActionType> ;
                                                   rdfs:comment "The Executable Action Type is the base class for actions that require executing generic programs on the system." ;
                                                   rdfs:label "Generic Executable" .


###  https://www.eclipse.org/ice/workflows#ExternalAgent
<https://www.eclipse.org/ice/workflows#ExternalAgent> rdf:type owl:Class ;
                                                      rdfs:subClassOf <https://www.eclipse.org/ice/workflows#Condition> ;
                                                      rdfs:comment "The External Agent Condition describes an action that waits conditionally on feedback from an external agent, including a human or an external service. Tasks can block themselves to wait on feedback, but in some cases an explicit task may exist for a user can that can be described and explicitly executed in the workflow." ;
                                                      rdfs:label "External Agent Condition" .


###  https://www.eclipse.org/ice/workflows#FortranFunction
<https://www.eclipse.org/ice/workflows#FortranFunction> rdf:type owl:Class ;
                                                        rdfs:subClassOf <https://www.eclipse.org/ice/workflows#LanguageInvocation> ;
                                                        rdfs:comment "The Fortran Function Action Type is the base class for actions that require executing a function in the Fortran programming language." ;
                                                        rdfs:label "Fortran Function" .


###  https://www.eclipse.org/ice/workflows#JavaClass
<https://www.eclipse.org/ice/workflows#JavaClass> rdf:type owl:Class ;
                                                  rdfs:subClassOf <https://www.eclipse.org/ice/workflows#LanguageInvocation> ;
                                                  rdfs:comment "The Java Class Action Type is the base class for actions that require executing a class in the Java programming language. Action Targets for this type should point to a single target method in the class that will create all necessary state and configure the system before executing. Thus, to execute a class Car, it may make sense to call a builder class such as \"CarBuilder.runCar\" instead." ;
                                                  rdfs:label "Java Class" .


###  https://www.eclipse.org/ice/workflows#LanguageInvocation
<https://www.eclipse.org/ice/workflows#LanguageInvocation> rdf:type owl:Class ;
                                                           rdfs:subClassOf <https://www.eclipse.org/ice/workflows#ActionType> ;
                                                           rdfs:comment "This action type represents actions to invocation language-specific calls or executions as part of the workflow. This could include, for example, executing a method on a native Java class, or a Fortran function or subroutine, or an R function." ;
                                                           rdfs:label "Language Invocation" .


###  https://www.eclipse.org/ice/workflows#Loop
<https://www.eclipse.org/ice/workflows#Loop> rdf:type owl:Class ;
                                             rdfs:subClassOf <https://www.eclipse.org/ice/workflows#Condition> ;
                                             rdfs:comment "The Loop describes an action that exits when a condition describing the end of a loop has been met. The loop executes over a range, and differs from a cyclic action type because the latter checks for the completion of a task cycle." ;
                                             rdfs:label "Loop" .


###  https://www.eclipse.org/ice/workflows#ParallelLoop
<https://www.eclipse.org/ice/workflows#ParallelLoop> rdf:type owl:Class ;
                                                     rdfs:subClassOf <https://www.eclipse.org/ice/workflows#Loop> ;
                                                     rdfs:comment "A Parallel Loop Condition indicates that the loop may be executed in parallel (i.e. - that the iterations of the loop are independent)." ;
                                                     rdfs:label "Parallel Loop" .


###  https://www.eclipse.org/ice/workflows#PythonScript
<https://www.eclipse.org/ice/workflows#PythonScript> rdf:type owl:Class ;
                                                     rdfs:subClassOf <https://www.eclipse.org/ice/workflows#LanguageInvocation> ;
                                                     rdfs:comment "The Python Script Action Type is the base class for actions that require executing a script in the Python programming language." ;
                                                     rdfs:label "Python Script" .


###  https://www.eclipse.org/ice/workflows#RESTfulService
<https://www.eclipse.org/ice/workflows#RESTfulService> rdf:type owl:Class ;
                                                       rdfs:subClassOf <https://www.eclipse.org/ice/workflows#WebService> ;
                                                       rdfs:comment "This action types describes Representational State Transfer (RESTful) web services." ;
                                                       rdfs:label "RESTful Web Service" .


###  https://www.eclipse.org/ice/workflows#SOAPService
<https://www.eclipse.org/ice/workflows#SOAPService> rdf:type owl:Class ;
                                                    rdfs:subClassOf <https://www.eclipse.org/ice/workflows#WebService> ;
                                                    rdfs:comment "This action types describes Simple Object Access Protocol (SOAP) web services." ;
                                                    rdfs:label "SOAP Web Service" .


###  https://www.eclipse.org/ice/workflows#ShellScript
<https://www.eclipse.org/ice/workflows#ShellScript> rdf:type owl:Class ;
                                                    rdfs:subClassOf <https://www.eclipse.org/ice/workflows#ActionType> ;
                                                    rdfs:comment "The Shell Script action type is for actions that require executing shell scripts on systems that support shells." ;
                                                    rdfs:label "Shell Script" .


###  https://www.eclipse.org/ice/workflows#StateChangeAction
<https://www.eclipse.org/ice/workflows#StateChangeAction> rdf:type owl:Class ;
                                                          rdfs:subClassOf <https://www.eclipse.org/ice/workflows#ConditionalAction> ;
                                                          rdfs:comment "A State Change is executed under the condition that a task experiences a state change." ;
                                                          rdfs:label "State Change" .


###  https://www.eclipse.org/ice/workflows#Task
<https://www.eclipse.org/ice/workflows#Task> rdf:type owl:Class ;
                                             rdfs:comment """Tasks are executed by workflows. They are modeled as the combination of an action and properties defining the way that action should be executed.

Tasks may also be assigned conditional actions that evaluate when a certain condition has been met based on the execution of the primary action with its properties.""" ;
                                             rdfs:label "Task" .


###  https://www.eclipse.org/ice/workflows#WSDLService
<https://www.eclipse.org/ice/workflows#WSDLService> rdf:type owl:Class ;
                                                    rdfs:subClassOf <https://www.eclipse.org/ice/workflows#WebService> ;
                                                    rdfs:comment "This action types describes Web Service Description Language (WSDL) web services." ;
                                                    rdfs:label "WSDL Web Service" .


###  https://www.eclipse.org/ice/workflows#WebService
<https://www.eclipse.org/ice/workflows#WebService> rdf:type owl:Class ;
                                                   rdfs:subClassOf <https://www.eclipse.org/ice/workflows#ActionType> ;
                                                   rdfs:comment "The Web Service Action Type is the base class for actions that require executing remote web services." ;
                                                   rdfs:label "Web Service" .


###  https://www.eclipse.org/ice/workflows#WorkflowDescription
<https://www.eclipse.org/ice/workflows#WorkflowDescription> rdf:type owl:Class ;
                                                            rdfs:subClassOf <https://www.eclipse.org/ice/data#Identifiable> ;
                                                            rdfs:comment "This class provides a description of the data and tasks that make up a workflow. It describes a collections of tasks that are executed to accomplish an activity with certain goals according to various properties and possibly using some data."@en ;
                                                            rdfs:label "Workflow Description"@en .


#################################################################
#    General axioms
#################################################################

[ rdf:type owl:AllDisjointClasses ;
  owl:members ( <https://www.eclipse.org/ice/workflows#BasicActionType>
                <https://www.eclipse.org/ice/workflows#Condition>
                <https://www.eclipse.org/ice/workflows#Executable>
                <https://www.eclipse.org/ice/workflows#LanguageInvocation>
                <https://www.eclipse.org/ice/workflows#ShellScript>
                <https://www.eclipse.org/ice/workflows#WebService>
              )
] .


[ rdf:type owl:AllDisjointClasses ;
  owl:members ( <https://www.eclipse.org/ice/workflows#BasicActionType>
                <https://www.eclipse.org/ice/workflows#Executable>
                <https://www.eclipse.org/ice/workflows#LanguageInvocation>
                <https://www.eclipse.org/ice/workflows#ShellScript>
                <https://www.eclipse.org/ice/workflows#WebService>
              )
] .


[ rdf:type owl:AllDisjointClasses ;
  owl:members ( <https://www.eclipse.org/ice/workflows#BooleanCondition>
                <https://www.eclipse.org/ice/workflows#Cycle>
                <https://www.eclipse.org/ice/workflows#ExternalAgent>
                <https://www.eclipse.org/ice/workflows#Loop>
              )
] .


[ rdf:type owl:AllDisjointClasses ;
  owl:members ( <https://www.eclipse.org/ice/workflows#FortranFunction>
                <https://www.eclipse.org/ice/workflows#JavaClass>
                <https://www.eclipse.org/ice/workflows#PythonScript>
              )
] .


[ rdf:type owl:AllDisjointClasses ;
  owl:members ( <https://www.eclipse.org/ice/workflows#RESTfulService>
                <https://www.eclipse.org/ice/workflows#SOAPService>
                <https://www.eclipse.org/ice/workflows#WSDLService>
              )
] .


###  Generated by the OWL API (version 5.1.14) https://github.com/owlcs/owlapi/
